add Vec

Arithmetization/ISigmaOne/HFS/Basic.lean
@@ -13,19 +13,19 @@ namespace LO.Arith
 
 open FirstOrder FirstOrder.Arith
 
-variable {M : Type*} [Zero M] [One M] [Add M] [Mul M] [LT M] [M ⊧ₘ* 𝐈𝚺₁]
+variable {V : Type*} [Zero V] [One V] [Add V] [Mul V] [LT V] [V ⊧ₘ* 𝐈𝚺₁]
 
-@[simp] lemma susbset_insert (x a : M) : a ⊆ insert x a := by intro z hz; simp [hz]
+@[simp] lemma susbset_insert (x a : V) : a ⊆ insert x a := by intro z hz; simp [hz]
 
-@[simp] lemma bitRemove_susbset (x a : M) : bitRemove x a ⊆ a := by intro z; simp
+@[simp] lemma bitRemove_susbset (x a : V) : bitRemove x a ⊆ a := by intro z; simp
 
-lemma lt_of_mem_dom {x y m : M} (h : ⟪x, y⟫ ∈ m) : x < m := lt_of_le_of_lt (by simp) (lt_of_mem h)
+lemma lt_of_mem_dom {x y m : V} (h : ⟪x, y⟫ ∈ m) : x < m := lt_of_le_of_lt (by simp) (lt_of_mem h)
 
-lemma lt_of_mem_rng {x y m : M} (h : ⟪x, y⟫ ∈ m) : y < m := lt_of_le_of_lt (by simp) (lt_of_mem h)
+lemma lt_of_mem_rng {x y m : V} (h : ⟪x, y⟫ ∈ m) : y < m := lt_of_le_of_lt (by simp) (lt_of_mem h)
 
 section under
 
-@[simp] lemma under_subset_under_of_le {i j : M} : under i ⊆ under j ↔ i ≤ j :=
+@[simp] lemma under_subset_under_of_le {i j : V} : under i ⊆ under j ↔ i ≤ j :=
   ⟨by intro h; by_contra hij
       have : j < i := by simpa using hij
       simpa using h (mem_under_iff.mpr this),
@@ -38,30 +38,30 @@ end under
 
 section sUnion
 
-lemma sUnion_exists_unique (s : M) :
-    ∃! u : M, ∀ x, (x ∈ u ↔ ∃ t ∈ s, x ∈ t) := by
+lemma sUnion_exists_unique (s : V) :
+    ∃! u : V, ∀ x, (x ∈ u ↔ ∃ t ∈ s, x ∈ t) := by
   have : 𝚺₁-Predicate fun x ↦ ∃ t ∈ s, x ∈ t := by definability
   exact finite_comprehension₁! this
     ⟨s, fun i ↦ by
       rintro ⟨t, ht, hi⟩; exact lt_trans (lt_of_mem hi) (lt_of_mem ht)⟩
 
-def sUnion (s : M) : M := Classical.choose! (sUnion_exists_unique s)
+def sUnion (s : V) : V := Classical.choose! (sUnion_exists_unique s)
 
 prefix:80 "⋃ʰᶠ " => sUnion
 
-@[simp] lemma mem_sUnion_iff {a b : M} : a ∈ ⋃ʰᶠ b ↔ ∃ c ∈ b, a ∈ c := Classical.choose!_spec (sUnion_exists_unique b) a
+@[simp] lemma mem_sUnion_iff {a b : V} : a ∈ ⋃ʰᶠ b ↔ ∃ c ∈ b, a ∈ c := Classical.choose!_spec (sUnion_exists_unique b) a
 
-@[simp] lemma sUnion_empty : (⋃ʰᶠ ∅ : M) = ∅ := mem_ext (by simp)
+@[simp] lemma sUnion_empty : (⋃ʰᶠ ∅ : V) = ∅ := mem_ext (by simp)
 
-lemma sUnion_lt_of_pos {a : M} (ha : 0 < a) : ⋃ʰᶠ a < a :=
+lemma sUnion_lt_of_pos {a : V} (ha : 0 < a) : ⋃ʰᶠ a < a :=
   lt_of_lt_log ha (by simp; intro i x hx hi; exact lt_of_lt_of_le (lt_of_mem hi) (le_log_of_mem hx))
 
-@[simp] lemma sUnion_le (a : M) : ⋃ʰᶠ a ≤ a := by
+@[simp] lemma sUnion_le (a : V) : ⋃ʰᶠ a ≤ a := by
   rcases zero_le a with (rfl | pos)
   · simp [←emptyset_def]
   · exact le_of_lt (sUnion_lt_of_pos pos)
 
-lemma sUnion_graph {u s : M} : u = ⋃ʰᶠ s ↔ ∀ x < u + s, (x ∈ u ↔ ∃ t ∈ s, x ∈ t) :=
+lemma sUnion_graph {u s : V} : u = ⋃ʰᶠ s ↔ ∀ x < u + s, (x ∈ u ↔ ∃ t ∈ s, x ∈ t) :=
   ⟨by rintro rfl; simp, by
     intro h; apply mem_ext
     intro x; simp
@@ -74,27 +74,27 @@ lemma sUnion_graph {u s : M} : u = ⋃ʰᶠ s ↔ ∀ x < u + s, (x ∈ u ↔ �
 def _root_.LO.FirstOrder.Arith.sUnionDef : 𝚺₀-Semisentence 2 := .mkSigma
   “u s | ∀ x < u + s, (x ∈ u ↔ ∃ t ∈' s, x ∈ t)” (by simp)
 
-lemma sUnion_defined : 𝚺₀-Function₁ ((⋃ʰᶠ ·) : M → M) via sUnionDef := by
+lemma sUnion_defined : 𝚺₀-Function₁ ((⋃ʰᶠ ·) : V → V) via sUnionDef := by
   intro v; simp [sUnionDef, sUnion_graph]
 
 @[simp] lemma sUnion_defined_iff (v) :
-    Semiformula.Evalbm M v sUnionDef.val ↔ v 0 = ⋃ʰᶠ v 1 := sUnion_defined.df.iff v
+    Semiformula.Evalbm V v sUnionDef.val ↔ v 0 = ⋃ʰᶠ v 1 := sUnion_defined.df.iff v
 
-instance sUnion_definable : DefinableFunction₁ ℒₒᵣ 𝚺₀ ((⋃ʰᶠ ·) : M → M) := Defined.to_definable _ sUnion_defined
+instance sUnion_definable : DefinableFunction₁ ℒₒᵣ 𝚺₀ ((⋃ʰᶠ ·) : V → V) := Defined.to_definable _ sUnion_defined
 
-instance sUnion_definable' (Γ) : DefinableFunction₁ ℒₒᵣ Γ ((⋃ʰᶠ ·) : M → M) := .of_zero sUnion_definable _
+instance sUnion_definable' (Γ) : DefinableFunction₁ ℒₒᵣ Γ ((⋃ʰᶠ ·) : V → V) := .of_zero sUnion_definable _
 
 end sUnion
 
 section union
 
-def union (a b : M) : M := ⋃ʰᶠ {a, b}
+def union (a b : V) : V := ⋃ʰᶠ {a, b}
 
-scoped instance : Union M := ⟨union⟩
+scoped instance : Union V := ⟨union⟩
 
-@[simp] lemma mem_cup_iff {a b c : M} : a ∈ b ∪ c ↔ a ∈ b ∨ a ∈ c := by simp [Union.union, union]
+@[simp] lemma mem_cup_iff {a b c : V} : a ∈ b ∪ c ↔ a ∈ b ∨ a ∈ c := by simp [Union.union, union]
 
-private lemma union_graph {u s t : M} : u = s ∪ t ↔ ∀ x < u + s + t, (x ∈ u ↔ x ∈ s ∨ x ∈ t) :=
+private lemma union_graph {u s t : V} : u = s ∪ t ↔ ∀ x < u + s + t, (x ∈ u ↔ x ∈ s ∨ x ∈ t) :=
   ⟨by rintro rfl; simp, by
     intro h; apply mem_ext
     intro x; simp
@@ -107,19 +107,19 @@ private lemma union_graph {u s t : M} : u = s ∪ t ↔ ∀ x < u + s + t, (x �
 def _root_.LO.FirstOrder.Arith.unionDef : 𝚺₀-Semisentence 3 := .mkSigma
   “∀[#0 < #1 + #2 + #3](#0 ∈ #1 ↔ #0 ∈ #2 ∨ #0 ∈ #3)” (by simp)
 
-lemma union_defined : 𝚺₀-Function₂ ((· ∪ ·) : M → M → M) via unionDef := by
+lemma union_defined : 𝚺₀-Function₂ ((· ∪ ·) : V → V → V) via unionDef := by
   intro v; simp [unionDef, union_graph]
 
 @[simp] lemma union_defined_iff (v) :
-    Semiformula.Evalbm M v unionDef.val ↔ v 0 = v 1 ∪ v 2 := union_defined.df.iff v
+    Semiformula.Evalbm V v unionDef.val ↔ v 0 = v 1 ∪ v 2 := union_defined.df.iff v
 
-instance union_definable : DefinableFunction₂ ℒₒᵣ 𝚺₀ ((· ∪ ·) : M → M → M) := Defined.to_definable _ union_defined
+instance union_definable : DefinableFunction₂ ℒₒᵣ 𝚺₀ ((· ∪ ·) : V → V → V) := Defined.to_definable _ union_defined
 
-instance union_definable' (Γ) : DefinableFunction₂ ℒₒᵣ Γ ((· ∪ ·) : M → M → M) := .of_zero union_definable _
+instance union_definable' (Γ) : DefinableFunction₂ ℒₒᵣ Γ ((· ∪ ·) : V → V → V) := .of_zero union_definable _
 
-lemma insert_eq_union_singleton (a s : M) : insert a s = {a} ∪ s := mem_ext (fun x ↦ by simp)
+lemma insert_eq_union_singleton (a s : V) : insert a s = {a} ∪ s := mem_ext (fun x ↦ by simp)
 
-@[simp] lemma union_polybound (a b : M) : a ∪ b ≤ 2 * (a + b) := le_iff_lt_succ.mpr
+@[simp] lemma union_polybound (a b : V) : a ∪ b ≤ 2 * (a + b) := le_iff_lt_succ.mpr
   <| lt_of_lt_log (by simp) (by
     simp; rintro i (hi | hi)
     · calc
@@ -131,24 +131,24 @@ lemma insert_eq_union_singleton (a s : M) : insert a s = {a} ∪ s := mem_ext (f
         _ < log (2 * (a + b)) := by simp [log_two_mul_of_pos (show 0 < a + b from by simp [pos_of_nonempty hi])]
         _ ≤ log (2 * (a + b) + 1) := log_monotone (by simp))
 
-instance : Bounded₂ ℒₒᵣ ((· ∪ ·) : M → M → M) := ⟨‘x y | 2 * (x + y)’, fun _ ↦ by simp⟩
+instance : Bounded₂ ℒₒᵣ ((· ∪ ·) : V → V → V) := ⟨‘x y | 2 * (x + y)’, fun _ ↦ by simp⟩
 
-lemma union_comm (a b : M) : a ∪ b = b ∪ a := mem_ext (by simp [or_comm])
+lemma union_comm (a b : V) : a ∪ b = b ∪ a := mem_ext (by simp [or_comm])
 
-@[simp] lemma union_succ_union_left (a b : M) : a ⊆ a ∪ b := by intro x hx; simp [hx]
+@[simp] lemma union_succ_union_left (a b : V) : a ⊆ a ∪ b := by intro x hx; simp [hx]
 
-@[simp] lemma union_succ_union_right (a b : M) : b ⊆ a ∪ b := by intro x hx; simp [hx]
+@[simp] lemma union_succ_union_right (a b : V) : b ⊆ a ∪ b := by intro x hx; simp [hx]
 
-@[simp] lemma union_succ_union_union_left (a b c : M) : a ⊆ a ∪ b ∪ c := by intro x hx; simp [hx]
+@[simp] lemma union_succ_union_union_left (a b c : V) : a ⊆ a ∪ b ∪ c := by intro x hx; simp [hx]
 
-@[simp] lemma union_succ_union_union_right (a b c : M) : b ⊆ a ∪ b ∪ c := by intro x hx; simp [hx]
+@[simp] lemma union_succ_union_union_right (a b c : V) : b ⊆ a ∪ b ∪ c := by intro x hx; simp [hx]
 
 end union
 
 section sInter
 
-lemma sInter_exists_unique (s : M) :
-    ∃! u : M, ∀ x, (x ∈ u ↔ s ≠ ∅ ∧ ∀ t ∈ s, x ∈ t) := by
+lemma sInter_exists_unique (s : V) :
+    ∃! u : V, ∀ x, (x ∈ u ↔ s ≠ ∅ ∧ ∀ t ∈ s, x ∈ t) := by
   have : 𝚺₁-Predicate fun x ↦ s ≠ ∅ ∧ ∀ t ∈ s, x ∈ t := by definability
   exact finite_comprehension₁! this
     ⟨s, fun i ↦ by
@@ -156,38 +156,38 @@ lemma sInter_exists_unique (s : M) :
       have : log s ∈ s := log_mem_of_pos <| pos_iff_ne_zero.mpr hs
       exact _root_.trans (lt_of_mem <| h (log s) this) (lt_of_mem this)⟩
 
-def sInter (s : M) : M := Classical.choose! (sInter_exists_unique s)
+def sInter (s : V) : V := Classical.choose! (sInter_exists_unique s)
 
 prefix:80 "⋂ʰᶠ " => sInter
 
-lemma mem_sInter_iff {x s : M} : x ∈ ⋂ʰᶠ s ↔ s ≠ ∅ ∧ ∀ t ∈ s, x ∈ t := Classical.choose!_spec (sInter_exists_unique s) x
+lemma mem_sInter_iff {x s : V} : x ∈ ⋂ʰᶠ s ↔ s ≠ ∅ ∧ ∀ t ∈ s, x ∈ t := Classical.choose!_spec (sInter_exists_unique s) x
 
-@[simp] lemma mem_sInter_iff_empty : ⋂ʰᶠ (∅ : M) = ∅ := mem_ext (by simp [mem_sInter_iff])
+@[simp] lemma mem_sInter_iff_empty : ⋂ʰᶠ (∅ : V) = ∅ := mem_ext (by simp [mem_sInter_iff])
 
-lemma mem_sInter_iff_of_pos {x s : M} (h : s ≠ ∅) : x ∈ ⋂ʰᶠ s ↔ ∀ t ∈ s, x ∈ t := by simp [mem_sInter_iff, h]
+lemma mem_sInter_iff_of_pos {x s : V} (h : s ≠ ∅) : x ∈ ⋂ʰᶠ s ↔ ∀ t ∈ s, x ∈ t := by simp [mem_sInter_iff, h]
 
 end sInter
 
 section inter
 
-def inter (a b : M) : M := ⋂ʰᶠ {a, b}
+def inter (a b : V) : V := ⋂ʰᶠ {a, b}
 
-scoped instance : Inter M := ⟨inter⟩
+scoped instance : Inter V := ⟨inter⟩
 
-@[simp] lemma mem_inter_iff {a b c : M} : a ∈ b ∩ c ↔ a ∈ b ∧ a ∈ c := by
+@[simp] lemma mem_inter_iff {a b c : V} : a ∈ b ∩ c ↔ a ∈ b ∧ a ∈ c := by
   simp [Inter.inter, inter, mem_sInter_iff_of_pos (s := {b, c}) (nonempty_iff.mpr ⟨b, by simp⟩)]
 
-lemma inter_comm (a b : M) : a ∩ b = b ∩ a := mem_ext (by simp [and_comm])
+lemma inter_comm (a b : V) : a ∩ b = b ∩ a := mem_ext (by simp [and_comm])
 
-lemma inter_eq_self_of_subset {a b : M} (h : a ⊆ b) :
+lemma inter_eq_self_of_subset {a b : V} (h : a ⊆ b) :
   a ∩ b = a := mem_ext (by simp; intro i hi; exact h hi)
 
 end inter
 
 section product
 
-lemma product_exists_unique (a b : M) :
-    ∃! u : M, ∀ x, (x ∈ u ↔ ∃ y ∈ a, ∃ z ∈ b, x = ⟪y, z⟫) := by
+lemma product_exists_unique (a b : V) :
+    ∃! u : V, ∀ x, (x ∈ u ↔ ∃ y ∈ a, ∃ z ∈ b, x = ⟪y, z⟫) := by
   have : 𝚺₁-Predicate fun x ↦ ∃ y ∈ a, ∃ z ∈ b, x = ⟪y, z⟫ := by definability
   exact finite_comprehension₁! this
     ⟨⟪log a, log b⟫ + 1, fun i ↦ by
@@ -195,24 +195,24 @@ lemma product_exists_unique (a b : M) :
       simp [lt_succ_iff_le]
       exact pair_le_pair (le_log_of_mem hy) (le_log_of_mem hz)⟩
 
-def product (a b : M) : M := Classical.choose! (product_exists_unique a b)
+def product (a b : V) : V := Classical.choose! (product_exists_unique a b)
 
 infixl:60 " ×ʰᶠ " => product
 
-lemma mem_product_iff {x a b : M} : x ∈ a ×ʰᶠ b ↔ ∃ y ∈ a, ∃ z ∈ b, x = ⟪y, z⟫ := Classical.choose!_spec (product_exists_unique a b) x
+lemma mem_product_iff {x a b : V} : x ∈ a ×ʰᶠ b ↔ ∃ y ∈ a, ∃ z ∈ b, x = ⟪y, z⟫ := Classical.choose!_spec (product_exists_unique a b) x
 
-lemma mem_product_iff' {x a b : M} : x ∈ a ×ʰᶠ b ↔ π₁ x ∈ a ∧ π₂ x ∈ b := by
+lemma mem_product_iff' {x a b : V} : x ∈ a ×ʰᶠ b ↔ π₁ x ∈ a ∧ π₂ x ∈ b := by
   simp [mem_product_iff]
   constructor
   · rintro ⟨y, hy, z, hz, rfl⟩; simp [*]
   · rintro ⟨h₁, h₂⟩; exact ⟨π₁ x, h₁, π₂ x, h₂, by simp⟩
 
-@[simp] lemma pair_mem_product_iff {x y a b : M} : ⟪x, y⟫ ∈ a ×ʰᶠ b ↔ x ∈ a ∧ y ∈ b := by simp [mem_product_iff']
+@[simp] lemma pair_mem_product_iff {x y a b : V} : ⟪x, y⟫ ∈ a ×ʰᶠ b ↔ x ∈ a ∧ y ∈ b := by simp [mem_product_iff']
 
-lemma pair_mem_product {x y a b : M} (hx : x ∈ a) (hy : y ∈ b) : ⟪x, y⟫ ∈ a ×ʰᶠ b := by
+lemma pair_mem_product {x y a b : V} (hx : x ∈ a) (hy : y ∈ b) : ⟪x, y⟫ ∈ a ×ʰᶠ b := by
   simp [mem_product_iff]; exact ⟨hx, hy⟩
 
-private lemma product_graph {u a b : M} : u = a ×ʰᶠ b ↔ ∀ x < u + (a + b + 1) ^ 2, (x ∈ u ↔ ∃ y ∈ a, ∃ z ∈ b, x = ⟪y, z⟫) :=
+private lemma product_graph {u a b : V} : u = a ×ʰᶠ b ↔ ∀ x < u + (a + b + 1) ^ 2, (x ∈ u ↔ ∃ y ∈ a, ∃ z ∈ b, x = ⟪y, z⟫) :=
   ⟨by rintro rfl x _; simp [mem_product_iff], by
     intro h
     apply mem_ext; intro x; simp [mem_product_iff]
@@ -225,22 +225,22 @@ private lemma product_graph {u a b : M} : u = a ×ʰᶠ b ↔ ∀ x < u + (a + b
 def _root_.LO.FirstOrder.Arith.productDef : 𝚺₀-Semisentence 3 := .mkSigma
   “u a b | ∀ x < u + (a + b + 1)², (x ∈ u ↔ ∃ y ∈' a, ∃ z ∈' b, !pairDef x y z)” (by simp)
 
-lemma product_defined : 𝚺₀-Function₂ ((· ×ʰᶠ ·) : M → M → M) via productDef := by
+lemma product_defined : 𝚺₀-Function₂ ((· ×ʰᶠ ·) : V → V → V) via productDef := by
   intro v; simp [productDef, product_graph]
 
 @[simp] lemma product_defined_iff (v) :
-    Semiformula.Evalbm M v productDef.val ↔ v 0 = v 1 ×ʰᶠ v 2 := product_defined.df.iff v
+    Semiformula.Evalbm V v productDef.val ↔ v 0 = v 1 ×ʰᶠ v 2 := product_defined.df.iff v
 
-instance product_definable : DefinableFunction₂ ℒₒᵣ 𝚺₀ ((· ×ʰᶠ ·) : M → M → M) := Defined.to_definable _ product_defined
+instance product_definable : DefinableFunction₂ ℒₒᵣ 𝚺₀ ((· ×ʰᶠ ·) : V → V → V) := Defined.to_definable _ product_defined
 
-instance product_definable' (Γ) : DefinableFunction₂ ℒₒᵣ Γ ((· ×ʰᶠ ·) : M → M → M) := .of_zero product_definable _
+instance product_definable' (Γ) : DefinableFunction₂ ℒₒᵣ Γ ((· ×ʰᶠ ·) : V → V → V) := .of_zero product_definable _
 
 end product
 
 section domain
 
-lemma domain_exists_unique (s : M) :
-    ∃! d : M, ∀ x, x ∈ d ↔ ∃ y, ⟪x, y⟫ ∈ s := by
+lemma domain_exists_unique (s : V) :
+    ∃! d : V, ∀ x, x ∈ d ↔ ∃ y, ⟪x, y⟫ ∈ s := by
   have : 𝚺₁-Predicate fun x ↦ ∃ y, ⟪x, y⟫ ∈ s :=
     DefinablePred.of_iff (fun x ↦ ∃ y < s, ⟪x, y⟫ ∈ s)
       (fun x ↦ ⟨by rintro ⟨y, hy⟩; exact ⟨y, lt_of_le_of_lt (le_pair_right x y) (lt_of_mem hy), hy⟩,
@@ -250,11 +250,11 @@ lemma domain_exists_unique (s : M) :
     this
     (⟨s, fun x ↦ by rintro ⟨y, hy⟩; exact lt_of_le_of_lt (le_pair_left x y) (lt_of_mem hy)⟩)
 
-def domain (s : M) : M := Classical.choose! (domain_exists_unique s)
+def domain (s : V) : V := Classical.choose! (domain_exists_unique s)
 
-lemma mem_domain_iff {x s : M} : x ∈ domain s ↔ ∃ y, ⟪x, y⟫ ∈ s := Classical.choose!_spec (domain_exists_unique s) x
+lemma mem_domain_iff {x s : V} : x ∈ domain s ↔ ∃ y, ⟪x, y⟫ ∈ s := Classical.choose!_spec (domain_exists_unique s) x
 
-private lemma domain_graph {u s : M} : u = domain s ↔ ∀ x < u + s, (x ∈ u ↔ ∃ y < s, ∃ z ∈ s, z = ⟪x, y⟫) :=
+private lemma domain_graph {u s : V} : u = domain s ↔ ∀ x < u + s, (x ∈ u ↔ ∃ y < s, ∃ z ∈ s, z = ⟪x, y⟫) :=
   ⟨by rintro rfl x _; simp [mem_domain_iff]
       exact ⟨by rintro ⟨y, hy⟩; exact ⟨y, lt_of_le_of_lt (le_pair_right x y) (lt_of_mem hy), hy⟩, by
         rintro ⟨y, _, hy⟩; exact ⟨y, hy⟩⟩,
@@ -269,19 +269,19 @@ private lemma domain_graph {u s : M} : u = domain s ↔ ∀ x < u + s, (x ∈ u 
 def _root_.LO.FirstOrder.Arith.domainDef : 𝚺₀-Semisentence 2 := .mkSigma
   “u s | ∀ x < u + s, (x ∈ u ↔ ∃ y < s, ∃ z ∈' s, !pairDef z x y)” (by simp)
 
-lemma domain_defined : 𝚺₀-Function₁ (domain : M → M) via domainDef := by
+lemma domain_defined : 𝚺₀-Function₁ (domain : V → V) via domainDef := by
   intro v; simp [domainDef, domain_graph]
 
 @[simp] lemma domain_defined_iff (v) :
-    Semiformula.Evalbm M v domainDef.val ↔ v 0 = domain (v 1) := domain_defined.df.iff v
+    Semiformula.Evalbm V v domainDef.val ↔ v 0 = domain (v 1) := domain_defined.df.iff v
 
-instance domain_definable : DefinableFunction₁ ℒₒᵣ 𝚺₀ (domain : M → M) := Defined.to_definable _ domain_defined
+instance domain_definable : DefinableFunction₁ ℒₒᵣ 𝚺₀ (domain : V → V) := Defined.to_definable _ domain_defined
 
-instance domain_definable' (Γ) : DefinableFunction₁ ℒₒᵣ Γ (domain : M → M) := .of_zero domain_definable _
+instance domain_definable' (Γ) : DefinableFunction₁ ℒₒᵣ Γ (domain : V → V) := .of_zero domain_definable _
 
-@[simp] lemma domain_empty : domain (∅ : M) = ∅ := mem_ext (by simp [mem_domain_iff])
+@[simp] lemma domain_empty : domain (∅ : V) = ∅ := mem_ext (by simp [mem_domain_iff])
 
-@[simp] lemma domain_union (a b : M) : domain (a ∪ b) = domain a ∪ domain b := mem_ext (by
+@[simp] lemma domain_union (a b : V) : domain (a ∪ b) = domain a ∪ domain b := mem_ext (by
   simp [mem_domain_iff]
   intro x; constructor
   · rintro ⟨y, (hy | hy)⟩
@@ -291,35 +291,35 @@ instance domain_definable' (Γ) : DefinableFunction₁ ℒₒᵣ Γ (domain : M 
     · exact ⟨y, Or.inl hy⟩
     · exact ⟨y, Or.inr hy⟩)
 
-@[simp] lemma domain_singleton (x y : M) : (domain {⟪x, y⟫} : M) = {x} := mem_ext (by simp [mem_domain_iff])
+@[simp] lemma domain_singleton (x y : V) : (domain {⟪x, y⟫} : V) = {x} := mem_ext (by simp [mem_domain_iff])
 
-@[simp] lemma domain_insert (x y s : M) : domain (insert ⟪x, y⟫ s) = insert x (domain s) := by simp [insert_eq_union_singleton]
+@[simp] lemma domain_insert (x y s : V) : domain (insert ⟪x, y⟫ s) = insert x (domain s) := by simp [insert_eq_union_singleton]
 
-@[simp] lemma domain_bound (s : M) : domain s ≤ 2 * s := le_iff_lt_succ.mpr
+@[simp] lemma domain_bound (s : V) : domain s ≤ 2 * s := le_iff_lt_succ.mpr
   <| lt_of_lt_log (by simp) (by
     simp [mem_domain_iff]; intro i x hix
     exact lt_of_le_of_lt (le_trans (le_pair_left i x) (le_log_of_mem hix))
       (by simp [log_two_mul_add_one_of_pos (pos_of_nonempty hix)]))
 
-instance : Bounded₁ ℒₒᵣ (domain : M → M) := ⟨‘x | 2 * x’, fun _ ↦ by simp⟩
+instance : Bounded₁ ℒₒᵣ (domain : V → V) := ⟨‘x | 2 * x’, fun _ ↦ by simp⟩
 
-lemma mem_domain_of_pair_mem {x y s : M} (h : ⟪x, y⟫ ∈ s) : x ∈ domain s := mem_domain_iff.mpr ⟨y, h⟩
+lemma mem_domain_of_pair_mem {x y s : V} (h : ⟪x, y⟫ ∈ s) : x ∈ domain s := mem_domain_iff.mpr ⟨y, h⟩
 
-lemma domain_subset_domain_of_subset {s t : M} (h : s ⊆ t) : domain s ⊆ domain t := by
+lemma domain_subset_domain_of_subset {s t : V} (h : s ⊆ t) : domain s ⊆ domain t := by
   intro x hx
   rcases mem_domain_iff.mp hx with ⟨y, hy⟩
   exact mem_domain_iff.mpr ⟨y, h hy⟩
 
-@[simp] lemma domain_eq_empty_iff_eq_empty {s : M} : domain s = ∅ ↔ s = ∅ :=
+@[simp] lemma domain_eq_empty_iff_eq_empty {s : V} : domain s = ∅ ↔ s = ∅ :=
   ⟨by simp [isempty_iff, mem_domain_iff]
       intro h x hx
       exact h (π₁ x) (π₂ x) (by simpa using hx), by rintro rfl; simp⟩
 
 /-
-@[simp] lemma domain_le_self {P : M → Prop}
+@[simp] lemma domain_le_self {P : V → Prop}
     (hempty : P ∅) (hinsert : ∀ s x, x ∉ s → P s → P (insert x s)) : ∀ x, P x := by {  }
 
-@[simp] lemma domain_le_self (P : M → Prop) (s : M) : domain s ≤ s := le_iff_lt_succ.mpr
+@[simp] lemma domain_le_self (P : V → Prop) (s : V) : domain s ≤ s := le_iff_lt_succ.mpr
 -/
 
 end domain
@@ -328,8 +328,8 @@ end domain
 
 section range
 
-lemma range_exists_unique (s : M) :
-    ∃! r : M, ∀ y, y ∈ r ↔ ∃ x, ⟪x, y⟫ ∈ s := by
+lemma range_exists_unique (s : V) :
+    ∃! r : V, ∀ y, y ∈ r ↔ ∃ x, ⟪x, y⟫ ∈ s := by
   have : 𝚺₁-Predicate fun y ↦ ∃ x, ⟪x, y⟫ ∈ s :=
     DefinablePred.of_iff (fun y ↦ ∃ x < s, ⟪x, y⟫ ∈ s)
       (fun y ↦ ⟨by rintro ⟨x, hy⟩; exact ⟨x, lt_of_le_of_lt (le_pair_left x y) (lt_of_mem hy), hy⟩,
@@ -340,11 +340,11 @@ lemma range_exists_unique (s : M) :
     (⟨s, fun y ↦ by rintro ⟨x, hx⟩; exact lt_of_le_of_lt (le_pair_right x y) (lt_of_mem hx)⟩)
 
 
-def range (s : M) : M := Classical.choose! (range_exists_unique s)
+def range (s : V) : V := Classical.choose! (range_exists_unique s)
 
-lemma mem_range_iff {y s : M} : y ∈ range s ↔ ∃ x, ⟪x, y⟫ ∈ s := Classical.choose!_spec (range_exists_unique s) y
+lemma mem_range_iff {y s : V} : y ∈ range s ↔ ∃ x, ⟪x, y⟫ ∈ s := Classical.choose!_spec (range_exists_unique s) y
 
-private lemma range_graph {s' s : M} : s' = range s ↔ ∀ y < s' + s, (y ∈ s' ↔ ∃ x < s, ∃ z ∈ s, z = ⟪x, y⟫) :=
+private lemma range_graph {s' s : V} : s' = range s ↔ ∀ y < s' + s, (y ∈ s' ↔ ∃ x < s, ∃ z ∈ s, z = ⟪x, y⟫) :=
   ⟨by rintro rfl y _; simp [mem_range_iff]
       exact ⟨by rintro ⟨x, hx⟩; exact ⟨x, lt_of_mem_dom hx, hx⟩, by
         rintro ⟨y, _, hy⟩; exact ⟨y, hy⟩⟩,
@@ -359,17 +359,17 @@ private lemma range_graph {s' s : M} : s' = range s ↔ ∀ y < s' + s, (y ∈ s
 def _root_.LO.FirstOrder.Arith.rangeDef : 𝚺₀-Semisentence 2 := .mkSigma
   “s' s | ∀ y < s' + s, (y ∈ s' ↔ ∃ x < s, ∃ z ∈' s, !pairDef z x y)” (by simp)
 
-lemma range_defined : 𝚺₀-Function₁ (range : M → M) via rangeDef := by
+lemma range_defined : 𝚺₀-Function₁ (range : V → V) via rangeDef := by
   intro v; simp [rangeDef, range_graph]
 
 @[simp] lemma range_defined_iff (v) :
-    Semiformula.Evalbm M v rangeDef.val ↔ v 0 = range (v 1) := range_defined.df.iff v
+    Semiformula.Evalbm V v rangeDef.val ↔ v 0 = range (v 1) := range_defined.df.iff v
 
-instance range_definable : DefinableFunction₁ ℒₒᵣ 𝚺₀ (range : M → M) := Defined.to_definable _ range_defined
+instance range_definable : DefinableFunction₁ ℒₒᵣ 𝚺₀ (range : V → V) := Defined.to_definable _ range_defined
 
-@[definability, simp] instance range_definable' (Γ) : DefinableFunction₁ ℒₒᵣ Γ (range : M → M) := .of_zero range_definable _
+@[definability, simp] instance range_definable' (Γ) : DefinableFunction₁ ℒₒᵣ Γ (range : V → V) := .of_zero range_definable _
 
-@[simp] lemma range_empty : range (∅ : M) = ∅ := mem_ext (by simp [mem_range_iff])
+@[simp] lemma range_empty : range (∅ : V) = ∅ := mem_ext (by simp [mem_range_iff])
 
 end range
 
@@ -377,16 +377,16 @@ end range
 
 section disjoint
 
-def Disjoint (s t : M) : Prop := s ∩ t = ∅
+def Disjoint (s t : V) : Prop := s ∩ t = ∅
 
-lemma Disjoint.iff {s t : M} : Disjoint s t ↔ ∀ x, x ∉ s ∨ x ∉ t := by simp [Disjoint, isempty_iff, imp_iff_not_or]
+lemma Disjoint.iff {s t : V} : Disjoint s t ↔ ∀ x, x ∉ s ∨ x ∉ t := by simp [Disjoint, isempty_iff, imp_iff_not_or]
 
-lemma Disjoint.not_of_mem {s t x : M} (hs : x ∈ s) (ht : x ∈ t) : ¬Disjoint s t := by
+lemma Disjoint.not_of_mem {s t x : V} (hs : x ∈ s) (ht : x ∈ t) : ¬Disjoint s t := by
   simp [Disjoint.iff, not_or]; exact ⟨x, hs, ht⟩
 
-lemma Disjoint.symm {s t : M} (h : Disjoint s t) : Disjoint t s := by simpa [Disjoint, inter_comm t s] using h
+lemma Disjoint.symm {s t : V} (h : Disjoint s t) : Disjoint t s := by simpa [Disjoint, inter_comm t s] using h
 
-@[simp] lemma Disjoint.singleton_iff {a : M} : Disjoint ({a} : M) s ↔ a ∉ s := by simp [Disjoint, isempty_iff]
+@[simp] lemma Disjoint.singleton_iff {a : V} : Disjoint ({a} : V) s ↔ a ∉ s := by simp [Disjoint, isempty_iff]
 
 end disjoint
 
@@ -394,11 +394,11 @@ end disjoint
 
 section mapping
 
-def IsMapping (m : M) : Prop := ∀ x ∈ domain m, ∃! y, ⟪x, y⟫ ∈ m
+def IsMapping (m : V) : Prop := ∀ x ∈ domain m, ∃! y, ⟪x, y⟫ ∈ m
 
 section
 
-private lemma isMapping_iff {m : M} :
+private lemma isMapping_iff {m : V} :
     IsMapping m ↔ ∃ d ≤ 2 * m, d = domain m ∧ ∀ x ∈ d, ∃ y < m, ⟪x, y⟫ ∈ m ∧ ∀ y' < m, ⟪x, y'⟫ ∈ m → y' = y :=
   ⟨by intro hm
       exact ⟨domain m, by simp, rfl, fun x hx ↦ by
@@ -411,31 +411,31 @@ private lemma isMapping_iff {m : M} :
 def _root_.LO.FirstOrder.Arith.isMappingDef : 𝚺₀-Semisentence 1 := .mkSigma
   “m | ∃ d <⁺ 2 * m, !domainDef d m ∧ ∀ x ∈' d, ∃ y < m, x ~[m] y ∧ ∀ y' < m, x ~[m] y' → y' = y” (by simp)
 
-lemma isMapping_defined : 𝚺₀-Predicate (IsMapping : M → Prop) via isMappingDef := by
+lemma isMapping_defined : 𝚺₀-Predicate (IsMapping : V → Prop) via isMappingDef := by
   intro v; simp [isMappingDef, isMapping_iff, lt_succ_iff_le]
 
 @[simp] lemma isMapping_defined_iff (v) :
-    Semiformula.Evalbm M v isMappingDef.val ↔ IsMapping (v 0) := isMapping_defined.df.iff v
+    Semiformula.Evalbm V v isMappingDef.val ↔ IsMapping (v 0) := isMapping_defined.df.iff v
 
-instance isMapping_definable : 𝚺₀-Predicate (IsMapping : M → Prop) := Defined.to_definable _ isMapping_defined
+instance isMapping_definable : 𝚺₀-Predicate (IsMapping : V → Prop) := Defined.to_definable _ isMapping_defined
 
-instance isMapping_definable' (Γ) : Γ-Predicate (IsMapping : M → Prop) := .of_zero isMapping_definable _
+instance isMapping_definable' (Γ) : Γ-Predicate (IsMapping : V → Prop) := .of_zero isMapping_definable _
 
 end
 
-lemma IsMapping.get_exists_uniq {m : M} (h : IsMapping m) {x : M} (hx : x ∈ domain m) : ∃! y, ⟪x, y⟫ ∈ m := h x hx
+lemma IsMapping.get_exists_uniq {m : V} (h : IsMapping m) {x : V} (hx : x ∈ domain m) : ∃! y, ⟪x, y⟫ ∈ m := h x hx
 
-def IsMapping.get {m : M} (h : IsMapping m) {x : M} (hx : x ∈ domain m) : M := Classical.choose! (IsMapping.get_exists_uniq h hx)
+def IsMapping.get {m : V} (h : IsMapping m) {x : V} (hx : x ∈ domain m) : V := Classical.choose! (IsMapping.get_exists_uniq h hx)
 
-@[simp] lemma IsMapping.get_mem {m : M} (h : IsMapping m) {x : M} (hx : x ∈ domain m) :
+@[simp] lemma IsMapping.get_mem {m : V} (h : IsMapping m) {x : V} (hx : x ∈ domain m) :
     ⟪x, h.get hx⟫ ∈ m := Classical.choose!_spec (IsMapping.get_exists_uniq h hx)
 
-lemma IsMapping.get_uniq {m : M} (h : IsMapping m) {x : M} (hx : x ∈ domain m) (hy : ⟪x, y⟫ ∈ m) : y = h.get hx :=
+lemma IsMapping.get_uniq {m : V} (h : IsMapping m) {x : V} (hx : x ∈ domain m) (hy : ⟪x, y⟫ ∈ m) : y = h.get hx :=
     (h x hx).unique hy (by simp)
 
-@[simp] lemma IsMapping.empty : IsMapping (∅ : M) := by intro x; simp
+@[simp] lemma IsMapping.empty : IsMapping (∅ : V) := by intro x; simp
 
-lemma IsMapping.union_of_disjoint_domain {m₁ m₂ : M}
+lemma IsMapping.union_of_disjoint_domain {m₁ m₂ : V}
     (h₁ : IsMapping m₁) (h₂ : IsMapping m₂) (disjoint : Disjoint (domain m₁) (domain m₂)) : IsMapping (m₁ ∪ m₂) := by
   intro x
   simp; rintro (hx | hx)
@@ -450,20 +450,20 @@ lemma IsMapping.union_of_disjoint_domain {m₁ m₂ : M}
       · by_contra; exact Disjoint.not_of_mem hx (mem_domain_of_pair_mem hy) disjoint.symm
       · exact h₂.get_uniq hx hy)
 
-@[simp] lemma IsMapping.singleton (x y : M) : IsMapping ({⟪x, y⟫} : M) := by
+@[simp] lemma IsMapping.singleton (x y : V) : IsMapping ({⟪x, y⟫} : V) := by
   intro x; simp; rintro rfl; exact ExistsUnique.intro y (by simp) (by rintro _ ⟨_, rfl⟩; simp)
 
-lemma IsMapping.insert {x y m : M}
+lemma IsMapping.insert {x y m : V}
     (h : IsMapping m) (disjoint : x ∉ domain m) : IsMapping (insert ⟪x, y⟫ m) := by
   simp [insert_eq_union_singleton]
   exact IsMapping.union_of_disjoint_domain (by simp) h (by simpa)
 
-lemma IsMapping.of_subset {m m' : M} (h : IsMapping m) (ss : m' ⊆ m) : IsMapping m' := fun x hx ↦ by
+lemma IsMapping.of_subset {m m' : V} (h : IsMapping m) (ss : m' ⊆ m) : IsMapping m' := fun x hx ↦ by
   rcases mem_domain_iff.mp hx with ⟨y, hy⟩
   have : ∃! y, ⟪x, y⟫ ∈ m := h x (domain_subset_domain_of_subset ss hx)
   exact ExistsUnique.intro y hy (fun y' hy' ↦ this.unique (ss hy') (ss hy))
 
-lemma IsMapping.uniq {m x y₁ y₂ : M} (h : IsMapping m) : ⟪x, y₁⟫ ∈ m → ⟪x, y₂⟫ ∈ m → y₁ = y₂ := fun h₁ h₂ ↦
+lemma IsMapping.uniq {m x y₁ y₂ : V} (h : IsMapping m) : ⟪x, y₁⟫ ∈ m → ⟪x, y₂⟫ ∈ m → y₁ = y₂ := fun h₁ h₂ ↦
   h x (mem_domain_iff.mpr ⟨y₁, h₁⟩) |>.unique h₁ h₂
 
 
@@ -473,37 +473,37 @@ end mapping
 
 section restriction
 
-lemma restr_exists_unique (f s : M) :
-    ∃! g : M, ∀ x, (x ∈ g ↔ x ∈ f ∧ π₁ x ∈ s) := by
+lemma restr_exists_unique (f s : V) :
+    ∃! g : V, ∀ x, (x ∈ g ↔ x ∈ f ∧ π₁ x ∈ s) := by
   have : 𝚺₁-Predicate fun x ↦ x ∈ f ∧ π₁ x ∈ s := by definability
   exact finite_comprehension₁! this
     ⟨f, fun i ↦ by rintro ⟨hi, _⟩; exact lt_of_mem hi⟩
 
-def restr (f s : M) : M := Classical.choose! (restr_exists_unique f s)
+def restr (f s : V) : V := Classical.choose! (restr_exists_unique f s)
 
 scoped infix:80 " ↾ " => restr
 
-lemma mem_restr_iff {x f s : M} : x ∈ f ↾ s ↔ x ∈ f ∧ π₁ x ∈ s := Classical.choose!_spec (restr_exists_unique f s) x
+lemma mem_restr_iff {x f s : V} : x ∈ f ↾ s ↔ x ∈ f ∧ π₁ x ∈ s := Classical.choose!_spec (restr_exists_unique f s) x
 
-@[simp] lemma pair_mem_restr_iff {x y f s : M} : ⟪x, y⟫ ∈ f ↾ s ↔ ⟪x, y⟫ ∈ f ∧ x ∈ s := by simp [mem_restr_iff]
+@[simp] lemma pair_mem_restr_iff {x y f s : V} : ⟪x, y⟫ ∈ f ↾ s ↔ ⟪x, y⟫ ∈ f ∧ x ∈ s := by simp [mem_restr_iff]
 
-@[simp] lemma restr_empty (f : M) : f ↾ ∅ = ∅ := mem_ext (by simp [mem_restr_iff])
+@[simp] lemma restr_empty (f : V) : f ↾ ∅ = ∅ := mem_ext (by simp [mem_restr_iff])
 
-@[simp] lemma restr_subset_self (f s : M) : f ↾ s ⊆ f := fun _ hx ↦ (mem_restr_iff.mp hx).1
+@[simp] lemma restr_subset_self (f s : V) : f ↾ s ⊆ f := fun _ hx ↦ (mem_restr_iff.mp hx).1
 
-@[simp] lemma restr_le_self (f s : M) : f ↾ s ≤ f := le_of_subset (by simp)
+@[simp] lemma restr_le_self (f s : V) : f ↾ s ≤ f := le_of_subset (by simp)
 
-lemma IsMapping.restr {m : M} (h : IsMapping m) (s : M) : IsMapping (m ↾ s) := h.of_subset (by simp)
+lemma IsMapping.restr {m : V} (h : IsMapping m) (s : V) : IsMapping (m ↾ s) := h.of_subset (by simp)
 
-lemma domain_restr (f s : M) : domain (f ↾ s) = domain f ∩ s :=
+lemma domain_restr (f s : V) : domain (f ↾ s) = domain f ∩ s :=
   mem_ext (by simp [mem_domain_iff, pair_mem_restr_iff, exists_and_right, mem_inter_iff])
 
-lemma domain_restr_of_subset_domain {f s : M} (h : s ⊆ domain f) : domain (f ↾ s) = s := by
+lemma domain_restr_of_subset_domain {f s : V} (h : s ⊆ domain f) : domain (f ↾ s) = s := by
   simp [domain_restr, inter_comm, inter_eq_self_of_subset h]
 
 end restriction
 
-theorem insert_induction {P : M → Prop} (hP : (Γ, 1)-Predicate P)
+theorem insert_induction {P : V → Prop} (hP : (Γ, 1)-Predicate P)
     (hempty : P ∅) (hinsert : ∀ a s, a ∉ s → P s → P (insert a s)) : ∀ s, P s :=
   order_induction_hh ℒₒᵣ Γ 1 hP <| by
     intro s IH
@@ -513,16 +513,16 @@ theorem insert_induction {P : M → Prop} (hP : (Γ, 1)-Predicate P)
         hinsert x (bitRemove x s) (by simp) (IH _ (bitRemove_lt_of_mem hx))
 
 @[elab_as_elim]
-lemma insert_induction_sigmaOne {P : M → Prop} (hP : 𝚺₁-Predicate P)
+lemma insert_induction_sigmaOne {P : V → Prop} (hP : 𝚺₁-Predicate P)
     (hempty : P ∅) (hinsert : ∀ a s, a ∉ s → P s → P (insert a s)) : ∀ s, P s :=
   insert_induction hP hempty hinsert
 
 @[elab_as_elim]
-lemma insert_induction_piOne {P : M → Prop} (hP : 𝚷₁-Predicate P)
+lemma insert_induction_piOne {P : V → Prop} (hP : 𝚷₁-Predicate P)
     (hempty : P ∅) (hinsert : ∀ a s, a ∉ s → P s → P (insert a s)) : ∀ s, P s :=
   insert_induction hP hempty hinsert
 
-theorem sigmaOne_skolem {R : M → M → Prop} (hP : 𝚺₁-Relation R) {s : M}
+theorem sigmaOne_skolem {R : V → V → Prop} (hP : 𝚺₁-Relation R) {s : V}
     (H : ∀ x ∈ s, ∃ y, R x y) : ∃ f, IsMapping f ∧ domain f = s ∧ ∀ x y, ⟪x, y⟫ ∈ f → R x y := by
   have : ∀ u, u ⊆ s → ∃ f, IsMapping f ∧ domain f = u ∧ ∀ x y, ⟪x, y⟫ ∈ f → R x y := by
     intro u hu
@@ -547,10 +547,10 @@ theorem sigmaOne_skolem {R : M → M → Prop} (hP : 𝚺₁-Relation R) {s : M}
         · exact hf x y h⟩
   exact this s (by rfl)
 
-theorem sigma₁_replacement {f : M → M} (hf : 𝚺₁-Function₁ f) (s : M) :
-    ∃! t : M, ∀ y, y ∈ t ↔ ∃ x ∈ s, y = f x := by
+theorem sigma₁_replacement {f : V → V} (hf : 𝚺₁-Function₁ f) (s : V) :
+    ∃! t : V, ∀ y, y ∈ t ↔ ∃ x ∈ s, y = f x := by
   have : ∀ x ∈ s, ∃ y, y = f x := by intro x _; exact ⟨f x, rfl⟩
-  have : ∃ F, IsMapping F ∧ domain F = s ∧ ∀ (x y : M), ⟪x, y⟫ ∈ F → y = f x :=
+  have : ∃ F, IsMapping F ∧ domain F = s ∧ ∀ (x y : V), ⟪x, y⟫ ∈ F → y = f x :=
     sigmaOne_skolem (by definability) this
   rcases this with ⟨F, _, rfl, hF⟩
   refine ExistsUnique.intro (range F) ?_ ?_
@@ -567,8 +567,8 @@ theorem sigma₁_replacement {f : M → M} (hf : 𝚺₁-Function₁ f) (s : M) 
     · rintro ⟨x, ⟨y, hxy⟩, rfl⟩; exact ⟨x, by rcases hF _ _ hxy; exact hxy⟩
     · rintro ⟨x, hxy⟩; exact ⟨x, ⟨y, hxy⟩, hF _ _ hxy⟩
 
-theorem sigma₁_replacement₂ {f : M → M → M} (hf : 𝚺₁-Function₂ f) (s₁ s₂ : M) :
-    ∃! t : M, ∀ y, y ∈ t ↔ ∃ x₁ ∈ s₁, ∃ x₂ ∈ s₂, y = f x₁ x₂ := by
+theorem sigma₁_replacement₂ {f : V → V → V} (hf : 𝚺₁-Function₂ f) (s₁ s₂ : V) :
+    ∃! t : V, ∀ y, y ∈ t ↔ ∃ x₁ ∈ s₁, ∃ x₂ ∈ s₂, y = f x₁ x₂ := by
   have : 𝚺₁-Function₁ (fun x ↦ f (π₁ x) (π₂ x)) := by definability
   exact (existsUnique_congr (by
       intro t; apply forall_congr'; intro y; apply iff_congr (by rfl)
@@ -576,6 +576,55 @@ theorem sigma₁_replacement₂ {f : M → M → M} (hf : 𝚺₁-Function₂ f)
       · rintro ⟨x, ⟨h₁, h₂⟩, rfl⟩; exact ⟨π₁ x, h₁, π₂ x, h₂, by rfl⟩
       · rintro ⟨x₁, h₁, x₂, h₂, rfl⟩; exact ⟨⟪x₁, x₂⟫, by simp [h₁, h₂]⟩)).mp
     (sigma₁_replacement this (s₁ ×ʰᶠ s₂))
+
+section fstIdx
+
+def fstIdx (p : V) : V := π₁ (p - 1)
+
+@[simp] lemma fstIdx_le_self (p : V) : fstIdx p ≤ p := le_trans (by simp [fstIdx]) (show p - 1 ≤ p by simp)
+
+def _root_.LO.FirstOrder.Arith.fstIdxDef : 𝚺₀-Semisentence 2 :=
+  .mkSigma “n p | ∃ p' <⁺ p, !subDef p' p 1 ∧ !pi₁Def n p'” (by simp)
+
+lemma fstIdx_defined : 𝚺₀-Function₁ (fstIdx : V → V) via fstIdxDef := by
+  intro v; simp [fstIdxDef]
+  constructor
+  · intro h; exact ⟨v 1 - 1, by simp, rfl, h⟩
+  · rintro ⟨_, _, rfl, h⟩; exact h
+
+@[simp] lemma eval_fstIdxDef (v) :
+    Semiformula.Evalbm V v fstIdxDef.val ↔ v 0 = fstIdx (v 1) := fstIdx_defined.df.iff v
+
+instance fstIdx_definable : 𝚺₀-Function₁ (fstIdx : V → V) := Defined.to_definable _ fstIdx_defined
+
+instance fstIdx_definable' (Γ) : Γ-Function₁ (fstIdx : V → V) := .of_zero fstIdx_definable _
+
+end fstIdx
+
+section sndIdx
+
+def sndIdx (p : V) : V := π₂ (p - 1)
+
+@[simp] lemma sndIdx_le_self (p : V) : sndIdx p ≤ p := le_trans (by simp [sndIdx]) (show p - 1 ≤ p by simp)
+
+def _root_.LO.FirstOrder.Arith.sndIdxDef : 𝚺₀-Semisentence 2 :=
+  .mkSigma “n p | ∃ p' <⁺ p, !subDef p' p 1 ∧ !pi₂Def n p'” (by simp)
+
+lemma sndIdx_defined : 𝚺₀-Function₁ (sndIdx : V → V) via sndIdxDef := by
+  intro v; simp [sndIdxDef]
+  constructor
+  · intro h; exact ⟨v 1 - 1, by simp, rfl, h⟩
+  · rintro ⟨_, _, rfl, h⟩; exact h
+
+@[simp] lemma eval_sndIdxDef (v) :
+    Semiformula.Evalbm V v sndIdxDef.val ↔ v 0 = sndIdx (v 1) := sndIdx_defined.df.iff v
+
+instance sndIdx_definable : 𝚺₀-Function₁ (sndIdx : V → V) := Defined.to_definable _ sndIdx_defined
+
+instance sndIdx_definable' (Γ) : Γ-Function₁ (sndIdx : V → V) := .of_zero sndIdx_definable _
+
+end sndIdx
+
 
 end LO.Arith
 
