Arithmetization/ISigmaOne/HFS/Vec.lean
@@ -1,0 +1,438 @@
+import Arithmetization.ISigmaOne.HFS.Fixpoint
+
+/-!
+
+# Vec
+
+-/
+
+noncomputable section
+
+namespace LO.Arith
+
+open FirstOrder FirstOrder.Arith
+
+variable {V : Type*} [Zero V] [One V] [Add V] [Mul V] [LT V] [V ⊧ₘ* 𝐈𝚺₁]
+
+namespace Nth
+
+def Phi (C : Set V) (pr : V) : Prop :=
+  (∃ v, pr = ⟪v, 0, fstIdx v⟫) ∨ (∃ v i x, pr = ⟪v, i + 1, x⟫ ∧ ⟪sndIdx v, i, x⟫ ∈ C)
+
+private lemma phi_iff (C pr : V) :
+    Phi {x | x ∈ C} pr ↔
+    (∃ v ≤ pr, ∃ fst ≤ v, fst = fstIdx v ∧ pr = ⟪v, 0, fst⟫) ∨
+    (∃ v ≤ pr, ∃ i ≤ pr, ∃ x ≤ pr, pr = ⟪v, i + 1, x⟫ ∧ ∃ snd ≤ v, snd = sndIdx v ∧ ∃ six < C, six = ⟪snd, i, x⟫ ∧ six ∈ C) := by
+  constructor
+  · rintro (⟨v, rfl⟩ | ⟨v, i, x, rfl, hC⟩)
+    · left; exact ⟨v, by simp, _, by simp, rfl, rfl⟩
+    · right; exact ⟨v, by simp,
+        i, le_trans (le_trans (by simp) (le_pair_left _ _)) (le_pair_right _ _),
+        x, le_trans (by simp) (le_pair_right _ _), rfl, _, by simp, rfl, _, lt_of_mem hC, rfl, hC⟩
+  · rintro (⟨v, _, _, _, rfl, rfl⟩ | ⟨v, _, i, _, x, _, rfl, _, _, rfl, _, _, rfl, hC⟩)
+    · left; exact ⟨v, rfl⟩
+    · right; exact ⟨v, i, x, rfl, hC⟩
+
+def blueprint : Fixpoint.Blueprint 0 where
+  core := .ofZero
+    (.mkSigma “pr C |
+    (∃ v <⁺ pr, ∃ fst <⁺ v, !fstIdxDef fst v ∧ !pair₃Def pr v 0 fst) ∨
+    (∃ v <⁺ pr, ∃ i <⁺ pr, ∃ x <⁺ pr, !pair₃Def pr v (i + 1) x ∧
+      ∃ snd <⁺ v, !sndIdxDef snd v ∧ ∃ six < C, !pair₃Def six snd i x ∧ six ∈ C)”
+    (by simp))
+    _
+
+def construction : Fixpoint.Construction V blueprint where
+  Φ := fun _ ↦ Phi
+  defined := .of_zero <| by intro v; simp [phi_iff]
+  monotone := by
+    rintro C C' hC _ x (h | ⟨v, i, x, rfl, h⟩)
+    · left; exact h
+    · right; exact ⟨v, i, x, rfl, hC h⟩
+
+instance : construction.Finite V where
+  finite := by
+    rintro C v x (h | ⟨v, i, x, rfl, h⟩)
+    · exact ⟨0, Or.inl h⟩
+    · exact ⟨⟪sndIdx v, i, x⟫ + 1, Or.inr ⟨v, i, x, rfl, h, by simp⟩⟩
+
+def Graph : V → Prop := construction.Fixpoint ![]
+
+section
+
+def graphDef : 𝚺₁-Semisentence 1 := blueprint.fixpointDef
+
+lemma graph_defined : 𝚺₁-Predicate (Graph : V → Prop) via graphDef :=
+  construction.fixpoint_defined
+
+instance graph_definable : 𝚺₁-Predicate (Graph : V → Prop) := Defined.to_definable _ graph_defined
+
+end
+
+/-- TODO: move-/
+@[simp] lemma zero_ne_add_one (x : V) : 0 ≠ x + 1 := ne_of_lt (by simp)
+
+lemma graph_case {pr : V} :
+    Graph pr ↔
+    (∃ v, pr = ⟪v, 0, fstIdx v⟫) ∨ (∃ v i x, pr = ⟪v, i + 1, x⟫ ∧ Graph ⟪sndIdx v, i, x⟫) :=
+  construction.case
+
+lemma graph_zero {v x : V} :
+    Graph ⟪v, 0, x⟫ ↔ x = fstIdx v := by
+  constructor
+  · intro h
+    rcases graph_case.mp h with (⟨v, h⟩ | ⟨v, i, x, h, _⟩)
+    · simp at h; rcases h with ⟨rfl, rfl, rfl⟩; rfl
+    · simp at h
+  · rintro rfl; exact graph_case.mpr <| Or.inl ⟨v, rfl⟩
+
+lemma graph_succ {v i x : V} :
+    Graph ⟪v, i + 1, x⟫ ↔ Graph ⟪sndIdx v, i, x⟫ := by
+  constructor
+  · intro h
+    rcases graph_case.mp h with (⟨v, h⟩ | ⟨v, i, x, h, hv⟩)
+    · simp at h
+    · simp at h; rcases h with ⟨rfl, rfl, rfl⟩; exact hv
+  · intro h; exact graph_case.mpr <| Or.inr ⟨v, i, x, rfl, h⟩
+
+lemma graph_exists (v i : V) : ∃ x, Graph ⟪v, i, x⟫ := by
+  suffices ∀ i' ≤ i, ∀ v' ≤ v, ∃ x, Graph ⟪v', i', x⟫ from this i (by simp) v (by simp)
+  intro i' hi'
+  induction i' using induction_iSigmaOne
+  · definability
+  case zero =>
+    intro v' _
+    exact ⟨fstIdx v', graph_case.mpr <| Or.inl ⟨v', rfl⟩⟩
+  case succ i' ih =>
+    intro v' hv'
+    rcases ih (le_trans le_self_add hi') (sndIdx v') (le_trans (by simp) hv') with ⟨x, hx⟩
+    exact ⟨x, graph_case.mpr <| Or.inr ⟨v', i', x, rfl, hx⟩⟩
+
+lemma graph_unique {v i x₁ x₂ : V} : Graph ⟪v, i, x₁⟫ → Graph ⟪v, i, x₂⟫ → x₁ = x₂ := by
+  induction i using induction_iPiOne generalizing v x₁ x₂
+  · definability
+  case zero =>
+    simp [graph_zero]
+    rintro rfl rfl; rfl
+  case succ i ih =>
+    simp [graph_succ]
+    exact ih
+
+lemma graph_existsUnique (v i : V) : ∃! x, Graph ⟪v, i, x⟫ := by
+  rcases graph_exists v i with ⟨x, hx⟩
+  exact ExistsUnique.intro x hx (fun y hy ↦ graph_unique hy hx)
+
+end Nth
+
+section nth
+
+open Nth
+
+def nth (v i : V) : V := Classical.choose! (graph_existsUnique v i)
+
+lemma nth_graph (v i : V) : Graph ⟪v, i, nth v i⟫ :=
+  Classical.choose!_spec (graph_existsUnique v i)
+
+lemma nth_eq_of_graph {v i x : V} (h : Graph ⟪v, i, x⟫) : nth v i = x := graph_unique (nth_graph v i) h
+
+lemma nth_zero (v : V) : nth v 0 = fstIdx v := nth_eq_of_graph (graph_zero.mpr rfl)
+
+lemma nth_succ (v i : V) : nth v (i + 1) = nth (sndIdx v) i := nth_eq_of_graph (graph_succ.mpr <| nth_graph _ _)
+
+instance : Cons V V := ⟨(⟪·, ·⟫ + 1)⟩
+
+scoped infixr:67 " ∷ " => cons
+
+syntax "?[" term,* "]" : term
+
+macro_rules
+  | `(?[$term:term, $terms:term,*]) => `(cons $term ?[$terms,*])
+  | `(?[$term:term]) => `(cons $term 0)
+  | `(?[]) => `(0)
+
+@[app_unexpander Cons.cons]
+def consUnexpander : Lean.PrettyPrinter.Unexpander
+  | `($_ $term ?[$terms,*]) => `(?[$term, $terms,*])
+  | `($_ $term 0) => `(?[$term])
+  | _ => throw ()
+
+lemma cons_def (x v : V) : x ∷ v = ⟪x, v⟫ + 1 := rfl
+
+@[simp] lemma fstIdx_cons (x v : V) : fstIdx (x ∷ v) = x := by simp [cons_def, fstIdx]
+
+@[simp] lemma sndIdx_cons (x v : V) : sndIdx (x ∷ v) = v := by simp [cons_def, sndIdx]
+
+lemma succ_eq_cons (x : V) : x + 1 = π₁ x ∷ π₂ x := by simp [cons_def]
+
+@[simp] lemma lt_cons (x v : V) : x < x ∷ v := by simp [cons_def, lt_succ_iff_le]
+
+@[simp] lemma lt_cons' (x v : V) : v < x ∷ v := by simp [cons_def, lt_succ_iff_le]
+
+@[simp] lemma zero_lt_cons (x v : V) : 0 < x ∷ v := by simp [cons_def]
+
+@[simp] lemma cons_ne_zero (x v : V) : x ∷ v ≠ 0 := by simp [cons_def]
+
+lemma nil_or_cons (z : V) : z = 0 ∨ ∃ x v, z = x ∷ v := by
+  rcases zero_or_succ z with (rfl | ⟨z, rfl⟩)
+  · left; rfl
+  · right; exact ⟨π₁ z, π₂ z, by simp [succ_eq_cons]⟩
+
+@[simp] lemma cons_inj (x₁ x₂ v₁ v₂ : V) :
+    x₁ ∷ v₁ = x₂ ∷ v₂ ↔ x₁ = x₂ ∧ v₁ = v₂ := by simp [cons_def]
+
+@[simp] lemma nth_cons_zero (x v : V) : nth (x ∷ v) 0 = x := by
+  simp [nth_zero]
+
+@[simp] lemma nth_cons_succ (x v i : V) : nth (x ∷ v) (i + 1) = nth v i := by
+  simp [nth_succ]
+
+lemma cons_induction (Γ) {P : V → Prop} (hP : (Γ, 1)-Predicate P)
+    (nil : P 0) (cons : ∀ x v, P v → P (x ∷ v)) : ∀ v, P v :=
+  order_induction_hh ℒₒᵣ Γ 1 hP (by
+    intro v ih
+    rcases nil_or_cons v with (rfl | ⟨x, v, rfl⟩)
+    · exact nil
+    · exact cons _ _ (ih v (by simp)))
+
+@[elab_as_elim]
+lemma cons_induction_sigma₁ {P : V → Prop} (hP : 𝚺₁-Predicate P)
+    (nil : P 0) (cons : ∀ x v, P v → P (x ∷ v)) : ∀ v, P v :=
+  cons_induction 𝚺 hP nil cons
+
+@[elab_as_elim]
+lemma cons_induction_pi₁ {P : V → Prop} (hP : 𝚷₁-Predicate P)
+    (nil : P 0) (cons : ∀ x v, P v → P (x ∷ v)) : ∀ v, P v :=
+  cons_induction 𝚷 hP nil cons
+
+section
+
+def _root_.LO.FirstOrder.Arith.nthDef : 𝚺₁-Semisentence 3 :=
+  .mkSigma “y v i | ∃ pr, !pair₃Def pr v i y ∧ !graphDef pr” (by simp)
+
+lemma nth_defined : 𝚺₁-Function₂ (nth : V → V → V) via nthDef := by
+  intro v; simp [nthDef, graph_defined.df.iff]
+  constructor
+  · intro h; rw [h]; exact nth_graph _ _
+  · intro h; simp [nth_eq_of_graph h]
+
+@[simp] lemma eval_nthDef (v) :
+    Semiformula.Evalbm V v nthDef.val ↔ v 0 = nth (v 1) (v 2) := nth_defined.df.iff v
+
+instance nth_definable : 𝚺₁-Function₂ (nth : V → V → V) := Defined.to_definable _ nth_defined
+
+instance nth_definable' (Γ) : (Γ, m + 1)-Function₂ (nth : V → V → V) := .of_sigmaOne nth_definable _ _
+
+def _root_.LO.FirstOrder.Arith.consDef : 𝚺₀-Semisentence 3 :=
+  .mkSigma “w x v | ∃ xv < w, !pairDef xv x v ∧ w = xv + 1” (by simp)
+
+lemma cons_defined : 𝚺₀-Function₂ (cons : V → V → V) via consDef := by
+  intro v; simp [consDef]
+  constructor
+  · intro h; rw [h]; exact ⟨_, by simp [cons_def], rfl, rfl⟩
+  · intro ⟨_, _, rfl, h⟩; exact h
+
+@[simp] lemma eval_cons (v) :
+    Semiformula.Evalbm V v consDef.val ↔ v 0 = v 1 ∷ v 2 := cons_defined.df.iff v
+
+instance cons_definable : 𝚺₀-Function₂ (cons : V → V → V) := Defined.to_definable _ cons_defined
+
+instance cons_definable' (Γ) : Γ-Function₂ (cons : V → V → V) := .of_zero cons_definable _
+
+end
+
+/-- TODO: move-/
+lemma pi₁_zero : π₁ (0 : V) = 0 := nonpos_iff_eq_zero.mp (pi₁_le_self 0)
+
+lemma pi₂_zero : π₂ (0 : V) = 0 := nonpos_iff_eq_zero.mp (pi₂_le_self 0)
+
+@[simp] lemma nth_zero_idx (i : V) : nth 0 i = 0 := by
+  induction i using induction_iSigmaOne
+  · definability
+  case zero => simp [nth_zero, fstIdx, pi₁_zero]
+  case succ i ih => simp [nth_succ, sndIdx, pi₂_zero, ih]
+
+lemma nth_lt_of_pos {v} (hv : 0 < v) (i : V) : nth v i < v := by
+  induction i using induction_iPiOne generalizing v
+  · definability
+  case zero =>
+    rcases zero_or_succ v with (rfl | ⟨v, rfl⟩)
+    · simp at hv
+    · simp [succ_eq_cons]
+  case succ i ih =>
+    rcases zero_or_succ v with (rfl | ⟨v, rfl⟩)
+    · simp at hv
+    · simp [succ_eq_cons v]
+      rcases eq_zero_or_pos (π₂ v) with (h | h)
+      · simp [h]
+      · exact lt_trans (ih h) (by simp)
+
+@[simp] lemma nth_le (v i : V) : nth v i ≤ v := by
+  rcases eq_zero_or_pos v with (h | h)
+  · simp [h]
+  · exact le_of_lt <| nth_lt_of_pos h i
+
+end nth
+
+namespace Len
+
+def Phi (C : Set V) (pr : V) : Prop :=
+  pr = ⟪0, 0⟫ ∨ (∃ v i, v ≠ 0 ∧ pr = ⟪v, i + 1⟫ ∧ ⟪sndIdx v, i⟫ ∈ C)
+
+private lemma phi_iff (C pr : V) :
+    Phi {x | x ∈ C} pr ↔
+    pr = ⟪0, 0⟫ ∨
+    (∃ v ≤ pr, ∃ i ≤ pr, v ≠ 0 ∧ pr = ⟪v, i + 1⟫ ∧ ∃ snd ≤ v, snd = sndIdx v ∧ ∃ six < C, six = ⟪snd, i⟫ ∧ six ∈ C) := by
+  constructor
+  · rintro (rfl | ⟨v, i, hv, rfl, hC⟩)
+    · left; rfl
+    · right; exact ⟨v, by simp,
+        i, le_trans le_self_add (le_pair_right _ _),
+        hv, rfl, _, by simp, rfl, _, lt_of_mem hC, rfl, hC⟩
+  · rintro (⟨v, _, _, _, rfl, rfl⟩ | ⟨v, _, i, _, hv, rfl, _, _, rfl, _, _, rfl, hC⟩)
+    · left; rfl
+    · right; exact ⟨v, i, hv, rfl, hC⟩
+
+def blueprint : Fixpoint.Blueprint 0 where
+  core := .ofZero
+    (.mkSigma “pr C |
+      !pairDef pr 0 0 ∨
+      (∃ v <⁺ pr, ∃ i <⁺ pr, v ≠ 0 ∧ !pairDef pr v (i + 1) ∧
+        ∃ snd <⁺ v, !sndIdxDef snd v ∧ ∃ six < C, !pairDef six snd i ∧ six ∈ C)”
+    (by simp))
+    _
+
+def construction : Fixpoint.Construction V blueprint where
+  Φ := fun _ ↦ Phi
+  defined := .of_zero <| by intro v; simp [phi_iff]
+  monotone := by
+    rintro C C' hC _ x (h | ⟨v, i, hv, rfl, h⟩)
+    · left; exact h
+    · right; exact ⟨v, i, hv, rfl, hC h⟩
+
+instance : construction.Finite V where
+  finite := by
+    rintro C v x (h | ⟨v, i, hv, rfl, h⟩)
+    · exact ⟨0, Or.inl h⟩
+    · exact ⟨⟪sndIdx v, i⟫ + 1, Or.inr ⟨v, i, hv, rfl, h, by simp⟩⟩
+
+def Graph : V → Prop := construction.Fixpoint ![]
+
+section
+
+def graphDef : 𝚺₁-Semisentence 1 := blueprint.fixpointDef
+
+lemma graph_defined : 𝚺₁-Predicate (Graph : V → Prop) via graphDef :=
+  construction.fixpoint_defined
+
+instance graph_definable : 𝚺₁-Predicate (Graph : V → Prop) := Defined.to_definable _ graph_defined
+
+end
+
+lemma graph_case {pr : V} :
+    Graph pr ↔ pr = ⟪0, 0⟫ ∨ (∃ v i, v ≠ 0 ∧ pr = ⟪v, i + 1⟫ ∧ Graph ⟪sndIdx v, i⟫) :=
+  construction.case
+
+lemma graph_zero {l : V} :
+    Graph ⟪0, l⟫ ↔ l = 0 := by
+  constructor
+  · intro h
+    rcases graph_case.mp h with (h | ⟨v, i, hv, h, _⟩)
+    · simp at h; rcases h with ⟨rfl, rfl⟩; rfl
+    · simp at h; rcases h with ⟨rfl, rfl⟩; simp at hv
+  · rintro rfl; exact graph_case.mpr <| Or.inl rfl
+
+lemma graph_succ {v x : V} :
+    Graph ⟪x ∷ v, l⟫ ↔ ∃ l', l = l' + 1 ∧ Graph ⟪v, l'⟫ := by
+  constructor
+  · intro h
+    rcases graph_case.mp h with (h | ⟨v, l, hv, h, hg⟩)
+    · simp at h
+    · simp at h; rcases h with ⟨rfl, rfl⟩; exact ⟨l, rfl, by simpa using hg⟩
+  · rintro ⟨l, rfl, h⟩; exact graph_case.mpr <| Or.inr ⟨x ∷ v, l, by simp, rfl, by simpa using h⟩
+
+lemma graph_exists (v : V) : ∃ l, Graph ⟪v, l⟫ := by
+  induction v using cons_induction_sigma₁
+  · definability
+  case nil =>
+    exact ⟨0, graph_zero.mpr rfl⟩
+  case cons x v ih =>
+    · rcases ih with ⟨l, hl⟩
+      exact ⟨l + 1, graph_succ.mpr ⟨l, rfl, hl⟩⟩
+
+lemma graph_unique {v l₁ l₂ : V} : Graph ⟪v, l₁⟫ → Graph ⟪v, l₂⟫ → l₁ = l₂ := by
+  induction v using cons_induction_pi₁ generalizing l₁ l₂
+  · definability
+  case nil =>
+    simp [graph_zero]; rintro rfl rfl; rfl
+  case cons x v ih =>
+    simp [graph_succ]
+    rintro l₁ rfl h₁ l₂ rfl h₂
+    rcases ih h₁ h₂; rfl
+
+lemma graph_existsUnique (v : V) : ∃! l, Graph ⟪v, l⟫ := by
+  rcases graph_exists v with ⟨l, hl⟩
+  exact ExistsUnique.intro l hl (fun y hy ↦ graph_unique hy hl)
+
+end Len
+
+section len
+
+open Len
+
+def len (v : V) : V := Classical.choose! (graph_existsUnique v)
+
+lemma len_graph (v : V) : Graph ⟪v, len v⟫ := Classical.choose!_spec (graph_existsUnique v)
+
+lemma len_eq_of_graph {v l : V} (h : Graph ⟪v, l⟫) : len v = l := graph_unique (len_graph v) h
+
+@[simp] lemma len_nil : len (0 : V) = 0 := len_eq_of_graph (graph_zero.mpr rfl)
+
+@[simp] lemma len_cons (x v : V) : len (x ∷ v) = len v + 1 := len_eq_of_graph (graph_succ.mpr ⟨_, rfl, len_graph v⟩)
+
+section
+
+def _root_.LO.FirstOrder.Arith.lenDef : 𝚺₁-Semisentence 2 :=
+  .mkSigma “l v | ∃ pr, !pairDef pr v l ∧ !graphDef pr” (by simp)
+
+lemma len_defined : 𝚺₁-Function₁ (len : V → V) via lenDef := by
+  intro v; simp [lenDef, graph_defined.df.iff]
+  constructor
+  · intro h; rw [h]; exact len_graph _
+  · intro h; rw [len_eq_of_graph h]
+
+@[simp] lemma eval_lenDef (v) :
+    Semiformula.Evalbm V v lenDef.val ↔ v 0 = len (v 1) := len_defined.df.iff v
+
+instance len_definable : 𝚺₁-Function₁ (len : V → V) := Defined.to_definable _ len_defined
+
+instance len_definable' (Γ) : (Γ, m + 1)-Function₁ (len : V → V) := .of_sigmaOne len_definable _ _
+
+end
+
+@[simp] lemma len_zero_iff_eq_nil {v : V} : len v = 0 ↔ v = 0 := by
+  rcases nil_or_cons v with (rfl | ⟨x, v, rfl⟩) <;> simp
+
+lemma nth_lt_len {v i : V} (hl : len v ≤ i) : nth v i = 0 := by
+  induction v using cons_induction_pi₁ generalizing i
+  · definability
+  case nil => simp
+  case cons x v ih =>
+    rcases zero_or_succ i with (rfl | ⟨i, rfl⟩)
+    · simp at hl
+    simpa using ih (by simpa using hl)
+
+lemma nth_ext {v₁ v₂ : V} (hl : len v₁ = len v₂) (H : ∀ i < len v₁, nth v₁ i = nth v₂ i) : v₁ = v₂ := by
+  induction v₁ using cons_induction_pi₁ generalizing v₂
+  · definability
+  case nil =>
+    exact Eq.symm <| len_zero_iff_eq_nil.mp (by simp [←hl])
+  case cons x₁ v₁ ih =>
+    rcases nil_or_cons v₂ with (rfl | ⟨x₂, v₂, rfl⟩)
+    · simp at hl
+    have hx : x₁ = x₂ := by simpa using H 0 (by simp)
+    have hv : v₁ = v₂ := ih (by simpa using hl) (by intro i hi; simpa using H (i + 1) (by simpa using hi))
+    simp [hx, hv]
+
+end len
+
+end LO.Arith
